iris/ProofSysUnlinkAUParts.v
@@ -176,21 +176,21 @@ Qed.
 
 Lemma su_au_nondir_node (n : fs_node) :
   fn_is_dir n = false ->
-  forall es, an_node (abs_of n) = ADir es -> dots_only es.
+  forall es, an_node (abs_row n) = ADir es -> dots_only es.
 Proof.
   intros Hd es Heq. exfalso. revert Heq.
-  rewrite /abs_of /abs_node /= Hd. case_decide; discriminate.
+  rewrite /abs_row /abs_node /= Hd. case_decide; discriminate.
 Qed.
 
 Lemma su_au_nondir_dec (n : fs_node) :
-  fn_is_dir n = false -> unl_dec (an_node (abs_of n)) = 0%nat.
+  fn_is_dir n = false -> unl_dec (an_node (abs_row n)) = 0%nat.
 Proof.
-  intros Hd. rewrite /abs_of /abs_node /= Hd. case_decide; reflexivity.
+  intros Hd. rewrite /abs_row /abs_node /= Hd. case_decide; reflexivity.
 Qed.
 
 Lemma su_au_dir_dec (n : fs_node) :
-  fn_is_dir n = true -> unl_dec (an_node (abs_of n)) = 1%nat.
-Proof. intros Hd. by rewrite /abs_of /abs_node /= Hd. Qed.
+  fn_is_dir n = true -> unl_dec (an_node (abs_row n)) = 1%nat.
+Proof. intros Hd. by rewrite /abs_row /abs_node /= Hd. Qed.
 
 (* the walked liveness facts, as [fn_nlink] bounds *)
 Lemma su_au_nl1 (dn : dinode) (bm : blkmap) (data : nat -> list (bv 8)) :
@@ -222,8 +222,8 @@ Lemma su_au_parent_row_era (dn dn' : dinode) (bm bm' : blkmap)
   dir_entries (era_node dn' bm' data')
     = delete nm (dir_entries (era_node dn bm data)) ->
   abs_of (era_node dn' bm' data')
-  = MkAnode (ADir (delete nm (dir_entries (era_node dn bm data))))
-            (fn_nlink (era_node dn bm data) - dec)%nat.
+  = Some (MkAnode (ADir (delete nm (dir_entries (era_node dn bm data))))
+                  (fn_nlink (era_node dn bm data) - dec)%nat).
 Proof.
   intros Hty Hty' Hnl Hents.
   apply (uf_parent_row _ _ nm dec); [| exact Hnl | exact Hents].
@@ -249,10 +249,10 @@ Lemma su_au_dir_dots (dn : dinode) (bm : blkmap)
   bv_unsigned (di_size dn) <= Z.of_nat MAXFILE * Z.of_nat BSIZE ->
   bv_unsigned (di_type dn) = T_DIR_z ->
   dir_dots_only dn data ->
-  forall es, an_node (abs_of (era_node dn bm data)) = ADir es -> dots_only es.
+  forall es, an_node (abs_row (era_node dn bm data)) = ADir es -> dots_only es.
 Proof.
   intros Hh Hb Hty Hdo es Heq.
-  rewrite (abs_of_dir _ (mkf_era_is_dir dn bm data Hty)) in Heq.
+  rewrite (abs_row_dir _ (mkf_era_is_dir dn bm data Hty)) in Heq.
   injection Heq as <-. exact (uf_dots_only dn bm data Hh Hb Hty Hdo).
 Qed.
 
